Example.v
@@ -1,0 +1,13 @@
+(* A tiny example of Coq code *)
+
+Section EXAMPLE.
+   Variables A B C : Prop.
+   Theorem example : (A -> B) -> (B -> C) -> A -> C.
+   Proof.
+       intros H H' HA. apply H'. apply H. assumption. 
+   Qed.
+
+   Definition example' : (A -> B) -> (B -> C) -> A -> C :=
+       fun (H : A -> B) (H' : B -> C) (HA : A) => H' (H HA).
+   Print example.
+End EXAMPLE.
